backup

type/isomorphism.v
@@ -41,6 +41,36 @@ Section gtth_ind_ref.
 
 End gtth_ind_ref.
 
+Inductive typ_gtth : list (option gtt) -> gtth -> gtt -> Prop := 
+  | gt_hol : forall n ctx gc, onth n ctx = Some gc -> typ_gtth ctx (gtth_hol n) gc
+  | gt_send : forall ctx p q xs ys, SList xs -> List.Forall2 (fun u v => (u = None /\ v = None) \/ 
+                                                (exists s g g', u = Some(s, g) /\ v = Some(s, g') /\ typ_gtth ctx g g')) xs ys -> 
+                                                typ_gtth ctx (gtth_send p q xs) (gtt_send p q ys).
+
+Section typ_gtth_ind_ref.
+  Variable P : list (option gtt) -> gtth -> gtt -> Prop.
+  Hypothesis P_hol : forall n ctx gc, onth n ctx = Some gc -> P ctx (gtth_hol n ) gc.
+  Hypothesis P_send : forall ctx p q xs ys, SList xs -> List.Forall2 (fun u v => (u = None /\ v = None) \/ 
+                                                 (exists s g g', u = Some(s, g) /\ v = Some(s, g') /\ P ctx g g')) xs ys -> 
+                                                 P ctx (gtth_send p q xs) (gtt_send p q ys).
+  
+  Fixpoint typ_gtth_ind_ref ctx G G' (a : typ_gtth ctx G G') {struct a} : P ctx G G'.
+  Proof.
+    refine (match a with 
+      | gt_hol n ctx gc Ha => P_hol n ctx gc Ha
+      | gt_send ctx p q xs ys Ha Hl => P_send ctx p q xs ys Ha _
+    end); try easy.
+    revert Hl. apply Forall2_mono.
+    intros. 
+    destruct H.
+    - left. easy.
+    - destruct H. destruct H. destruct H. destruct H. destruct H0. subst.
+      right. exists x0. exists x1. exists x2. split. easy. split. easy. 
+      apply typ_gtth_ind_ref; try easy.
+  Qed.
+
+End typ_gtth_ind_ref.
+
 Definition balancedG (G : global) := forall G w w' p q gn,
   gttmap G w None gn -> gttmap G (w ++ w') None (gnode_pq p q) -> 
   (exists k, forall w', gttmap G (w ++ w') None (gnode_end) \/ 
@@ -55,3 +85,7 @@ Definition wfgT G := wfG G /\ (forall n, exists m, guardG n m G) /\ balancedG G.
 Definition wfgC G := exists G', gttTC G' G /\ wfG G' /\ (forall n, exists m, guardG n m G') /\ balancedG G'. 
 
 Definition wfC T := exists T', lttTC T' T /\ wfL T' /\ (forall n, exists m, guardL n m T').
+
+
+
+
