type/projection.v
@@ -1,7 +1,7 @@
 From mathcomp Require Import ssreflect.seq all_ssreflect.
 From Paco Require Import paco pacotac.
 From SST Require Export src.expressions src.header type.global type.local type.isomorphism.
-Require Import List String Coq.Arith.PeanoNat Relations. 
+Require Import List String Coq.Arith.PeanoNat Relations.
 Import ListNotations. 
 
 Inductive isgParts : part -> global -> Prop := 
@@ -13,12 +13,13 @@ Inductive isgParts : part -> global -> Prop :=
 Definition isgPartsC (pt : part) (G : gtt) : Prop := 
     exists G', gttTC G' G /\ isgParts pt G'.
 
-Fixpoint isMerge (t : ltt) (lis : list (option ltt)) : Prop := 
-  match lis with 
-    | Some x :: xs => t = x /\ isMerge t xs
-    | None   :: xs => isMerge t xs
-    | []    => True 
-  end.
+Inductive ishParts : part -> gtth -> Prop := 
+  | ha_sendp : forall p q l, ishParts p (gtth_send p q l)
+  | ha_sendq : forall p q l, ishParts q (gtth_send p q l)
+  | ha_sendr : forall p q r n s g lis, p <> r -> q <> r -> onth n lis = Some (s, g) -> ishParts r g -> ishParts r (gtth_send p q lis).
+
+Definition isMerge (t : ltt) (lis : list (option ltt)) : Prop := 
+  List.Forall (fun u => u = None \/ (exists t', u = Some t' /\ t = t')) lis /\ SList lis.
 
 Variant projection (R: gtt -> part -> ltt -> Prop): gtt -> part -> ltt -> Prop :=
   | proj_end : forall g r, 
@@ -52,6 +53,9 @@ Proof. unfold monotone3.
        - try easy.
 Admitted.
 
+Lemma gttT_mon : monotone2 gttT.
+Admitted.
+
 Lemma pmergeCR: forall G r,
           projectionC G r ltt_end ->
           (isgPartsC r G -> False).
@@ -80,8 +84,462 @@ Variant gttstep (R: gtt -> gtt -> part -> part -> nat -> Prop): gtt -> gtt -> pa
 
 Definition gttstepC g1 g2 p q n := paco5 gttstep bot5 g1 g2 p q n. 
 
-Lemma wfgC_after_step : forall G G' p q n, gttstepC G G' p q n -> wfgC G'.
+Lemma proj_inj [G p T T'] :  projectionC G p T -> projectionC G p T' -> T = T'.
+Admitted.
+
+
+Lemma _a_29_10 : forall G p q PT S T n,
+    projectionC G p PT ->
+    subtypeC (ltt_send q (extendLis n (Some (S, T)))) PT ->
+    exists (xs : list (option (sort * ltt))) (Sk : sort) (Tk : ltt), projectionC G p (ltt_send q xs) /\ 
+    onth n xs = Some(Sk, Tk) /\ subsort S Sk /\ subtypeC T Tk.
+Proof.
+  intros.
+  specialize(subtype_send PT q (extendLis n (Some (S, T))) H0); intros.
+  destruct H1. subst.
+  specialize(subtype_send_inv q (extendLis n (Some (S,T))) x H0); intros.
+  exists x.
+  assert (exists Sk Tk, onth n x = Some (Sk, Tk) /\ subsort S Sk /\ subtypeC T Tk).
+  {
+    clear H0. clear H. revert G p q S T x H1.
+    induction n; intros; try easy.
+    - destruct x; try easy.
+      simpl in *. inversion H1. subst. destruct H3; try easy.
+      destruct H. destruct H. destruct H. destruct H. destruct H. destruct H0. destruct H2.
+      inversion H. subst.
+      exists x1. exists x3. try easy.
+    - destruct x; try easy. apply IHn; try easy.
+      inversion H1; try easy.
+  }
+  destruct H2. destruct H2. destruct H2. destruct H3.
+  exists x0. exists x1. try easy.
+Qed.
+
+Lemma _a_29_11 : forall G p q x,
+    wfgC G ->
+    projectionC G p (ltt_send q x) ->
+    exists G' ctxJ, 
+      typ_gtth ctxJ G' G /\ (ishParts p G' -> False) /\
+      List.Forall (fun u => u = None \/ (exists g lsg, u = Some g /\ g = gtt_send p q lsg /\
+        List.Forall2 (fun u v => (u = None /\ v = None) \/ (exists s t g', u = Some(s, g') /\ v = Some(s, t) /\
+          projectionC g' p t
+        )) lsg x 
+      )) ctxJ.
+Proof.
+    intros.
+Admitted.
+
+Lemma some_onth_implies_In {A} : forall n (ctxG : list (option A)) G,
+    onth n ctxG = Some G -> In (Some G) ctxG.
+Proof.
+  induction n; intros; try easy.
+  - destruct ctxG; try easy. simpl in *.
+    left. easy.
+  - destruct ctxG; try easy. simpl in *.
+    right. apply IHn; try easy.
+Qed.
+
+Lemma _a_29_1314 : forall G G' p q QT xs ctxG x,
+    Forall
+        (fun u : option gtt =>
+         u = None \/
+         (exists (g : gtt) (lsg : seq.seq (option (sort * gtt))),
+            u = Some g /\
+            g = gtt_send p q lsg /\
+            Forall2
+              (fun (u0 : option (sort * gtt)) (v : option (sort * ltt)) =>
+               u0 = None /\ v = None \/
+               (exists (s : sort) (t : ltt) (g' : gtt),
+                  u0 = Some (s, g') /\ v = Some (s, t) /\ projectionC g' p t)) lsg x))
+        ctxG -> 
+  typ_gtth ctxG G' G ->
+  (ishParts p G' -> False) ->
+  projectionC G q QT ->
+  subtypeC (ltt_recv p xs) QT -> 
+  exists ys, projectionC G q (ltt_recv p ys) /\ List.Forall2 (fun u v => (u = None /\ v = None) \/ (exists s t t', u = Some(s, t) /\ v = Some(s, t'))) ys x.
+Proof.
+  
+Admitted.
+
+Lemma _a_29_part_helper_recv : forall n ys1 x4 p ys,
+    onth n ys1 = Some x4 ->
+    isMerge (ltt_recv p ys) ys1 -> 
+    exists ys1', x4 = ltt_recv p ys1'.
 Proof.
 Admitted.
+
+Lemma _a_29_part_helper_send : forall n ys2 x3 q x,
+    onth n ys2 = Some x3 ->
+    isMerge (ltt_send q x) ys2 ->
+    exists ys2', x3 = ltt_send q ys2'.
+Proof.
+Admitted.
+
+Lemma _a_29_part : forall ctxG G' G p q x ys,
+    typ_gtth ctxG G' G -> 
+    projectionC G p (ltt_send q x) ->
+    projectionC G q (ltt_recv p ys) ->
+    (ishParts p G' -> False) -> 
+    (ishParts q G' -> False).
+Proof.
+    intros ctxG G'. revert ctxG.
+    induction G' using gtth_ind_ref; intros; try easy.
+    rename p into r. rename q into s. rename p0 into p. rename q0 into q.
+    inversion H0. subst.
+    inversion H4; try easy. 
+    - subst.
+      pinversion H2; try easy. subst.
+      unfold wfgC in H12. destruct H12. destruct H5. punfold H5. 
+      apply gttT_mon. apply proj_mon.
+    - subst. 
+      pinversion H2; try easy. subst.
+      apply H3. constructor.
+      apply proj_mon.
+    - subst.
+      specialize(some_onth_implies_In n xs (s0, g) H13); intros.
+      specialize(Forall_forall (fun u : option (sort * gtth) =>
+       u = None \/
+       (exists (s : sort) (g : gtth),
+          u = Some (s, g) /\
+          (forall (ctxG : seq.seq (option gtt)) (G : gtt) (p q : string)
+             (x ys : seq.seq (option (sort * ltt))),
+           typ_gtth ctxG g G ->
+           projectionC G p (ltt_send q x) ->
+           projectionC G q (ltt_recv p ys) ->
+           (ishParts p g -> False) -> ishParts q g -> False))) xs); intros.
+    destruct H6. specialize(H6 H). clear H H7.
+    specialize(H6 (Some (s0, g)) H5).
+    destruct H6; try easy.
+    destruct H. destruct H. destruct H.
+    inversion H. subst. clear H.
+    case_eq (eqb p s); intros; try easy.
+    - assert (p = s). apply eqb_eq; easy. subst. apply H3. constructor.
+    case_eq (eqb p r); intros; try easy.
+    - assert (p = r). apply eqb_eq; easy. subst. apply H3. constructor.
+    assert (p <> s). apply eqb_neq; try easy.
+    assert (p <> r). apply eqb_neq; try easy.
+    assert (ishParts p x1 -> False). 
+    {
+      intros. apply H3.
+      apply ha_sendr with (n := n) (s := x0) (g := x1); try easy.
+    }
+    assert (exists g', typ_gtth ctxG x1 g' /\ onth n ys0 = Some (x0, g')).
+    {
+      clear H2 H1 H0 H3 H4 H10 H8 H12 H5 H14 H6 H H7 H9 H15 H16. clear p q r s.
+      clear x ys.
+      revert H11 H13. revert xs ctxG ys0 x0 x1.
+      induction n; intros; try easy.
+      - destruct xs; try easy. 
+        destruct ys0; try easy.
+        inversion H11. simpl in *. subst.
+        destruct H2; try easy. destruct H. destruct H. destruct H. destruct H. destruct H0.
+        inversion H. subst.
+        exists x3; try easy.
+      - destruct xs; try easy.
+        destruct ys0; try easy.
+        apply IHn with (xs := xs) (ys0 := ys0) (x0 := x0); try easy.
+        inversion H11. easy.
+    }
+    destruct H17. 
+    specialize(H6 ctxG x2 p q).
+    pinversion H2; try easy. subst.
+    pinversion H1; try easy. subst. clear H25 H32 H30 H31. destruct H17.
+    assert (exists t t', projectionC x2 p t /\ projectionC x2 q t' /\ onth n ys2 = Some t /\ onth n ys1 = Some t').
+    {
+      clear H2 H1 H0 H3 H4 H10 H8 H12 H5 H14 H13 H6 H H7 H9 H15 H16 H17 H21 H22 H23 H24 H9 H26 H27 H36 H29 H11.
+      clear r s x1 x ys xs ctxG.
+      revert H18 H28 H35. revert p q x0 x2 ys0 ys1 ys2.
+      induction n; intros; try easy.
+      - destruct ys0; try easy.
+        destruct ys1; try easy.
+        destruct ys2; try easy.
+        simpl in *.
+        inversion H28. subst. inversion H35. subst. clear H28 H35.
+        destruct H2; try easy. destruct H. destruct H. destruct H. destruct H. destruct H0. inversion H. subst.
+        destruct H3; try easy. destruct H0. destruct H0. destruct H0. destruct H0. destruct H2. inversion H0. subst.
+        pclearbot. exists x4. exists x3. easy.
+      - destruct ys0; try easy.
+        destruct ys1; try easy.
+        destruct ys2; try easy.
+        simpl in *.
+        inversion H28. subst. inversion H35. subst. clear H28 H35.
+        apply IHn with (x0 := x0) (ys0 := ys0) (ys1 := ys1) (ys2 := ys2); try easy.
+    }
+    destruct H19. destruct H19. destruct H19. destruct H20. destruct H25.
+    specialize(_a_29_part_helper_recv n ys1 x4 p ys H30 H29); intros. destruct H31. subst.
+    specialize(_a_29_part_helper_send n ys2 x3 q x H25 H36); intros. destruct H31. subst.
+    specialize(H6 x4 x5). apply H6; try easy.
+    apply proj_mon.
+    apply proj_mon.
+Qed.
+
+Lemma _a_29_16 : forall G' ctxG G p q ys x, 
+    projectionC G q (ltt_recv p ys) -> 
+    Forall
+          (fun u : option gtt =>
+           u = None \/
+           (exists (g : gtt) (lsg : seq.seq (option (sort * gtt))),
+              u = Some g /\
+              g = gtt_send p q lsg /\
+              Forall2
+                (fun (u0 : option (sort * gtt)) (v : option (sort * ltt)) =>
+                 u0 = None /\ v = None \/
+                 (exists (s : sort) (t : ltt) (g' : gtt),
+                    u0 = Some (s, g') /\ v = Some (s, t) /\ projectionC g' p t)) lsg x)) ctxG ->
+    (ishParts p G' -> False) ->
+    (ishParts q G' -> False) -> 
+    typ_gtth ctxG G' G -> 
+    Forall
+          (fun u : option gtt =>
+           u = None \/
+           (exists (g : gtt) (lsg : seq.seq (option (sort * gtt))),
+              u = Some g /\
+              g = gtt_send p q lsg /\
+              Forall2
+                (fun (u0 : option (sort * gtt)) (v : option (sort * ltt)) =>
+                 u0 = None /\ v = None \/
+                 (exists (s : sort) (t : ltt) (g' : gtt),
+                    u0 = Some (s, g') /\ v = Some (s, t) /\ projectionC g' p t)) lsg x /\
+              Forall2
+                (fun u v => (u = None /\ v = None) \/ 
+                 (exists s t g', u = Some (s, g') /\ v = Some (s, t) /\ projectionC g' q t)) lsg ys
+              )) ctxG.
+Proof.
+  
+  
+Admitted.
+
+
+Lemma _a_29_helper : forall n x Sk Tk lsg p,
+    onth n x = Some (Sk, Tk) ->
+    Forall2 
+        (fun (u0 : option (sort * gtt)) (v : option (sort * ltt)) =>
+         u0 = None /\ v = None \/
+         (exists (s : sort) (t : ltt) (g' : gtt),
+            u0 = Some (s, g') /\ v = Some (s, t) /\ projectionC g' p t)) lsg x ->
+    exists Glsg, onth n lsg = Some (Sk, Glsg) /\ projectionC Glsg p Tk.
+Proof.
+  induction n; intros; try easy.
+  - destruct x; try easy.
+    destruct lsg; try easy.
+    simpl in *. subst.
+    inversion H0. subst. destruct H3; try easy. destruct H. destruct H. destruct H. destruct H. destruct H1. inversion H1. subst.
+    exists x2. split; try easy.
+  - destruct x; try easy. destruct lsg; try easy.
+    inversion H0. subst.
+    simpl in *. apply IHn with (x := x); try easy.
+Qed.
+
+Lemma _a_29_helper2 : forall lsg SI x p,
+      Forall2
+        (fun (u0 : option (sort * gtt)) (v : option (sort * ltt)) =>
+         u0 = None /\ v = None \/
+         (exists (s : sort) (t : ltt) (g' : gtt),
+            u0 = Some (s, g') /\ v = Some (s, t) /\ projectionC g' p t)) lsg x ->
+      Forall2
+        (fun (u : option sort) (v : option (sort * ltt)) =>
+         u = None /\ v = None \/
+         (exists (s : sort) (t : ltt), u = Some s /\ v = Some (s, t))) SI x ->
+      Forall2
+        (fun (u : option (sort * gtt)) (v : option sort) =>
+         u = None /\ v = None \/
+         (exists (s : sort) (g' : gtt), u = Some (s, g') /\ v = Some s)) lsg SI.
+Proof.
+  induction lsg; intros; try easy.
+  - destruct x; try easy.
+    destruct SI; try easy.
+  - destruct x; try easy.
+    destruct SI; try easy.
+    inversion H0. subst. clear H0. inversion H. subst. clear H.
+    constructor.
+    - destruct H4. left. destruct H. subst. destruct H3; try easy. destruct H. destruct H. destruct H.
+      destruct H. destruct H0. easy.
+    - destruct H. destruct H. destruct H. subst.
+      destruct H3; try easy. destruct H. destruct H. destruct H. destruct H. destruct H0.
+      inversion H0. subst. right.
+      exists x2. exists x4. split; try easy.
+  - apply IHlsg with (x := x) (p := p); try easy.
+Qed.
+
+Lemma _a_29_helper3 : forall n lsg x0 Sk ys q,
+    onth n lsg = Some(Sk, x0) -> 
+    Forall2
+          (fun (u0 : option (sort * gtt)) (v : option (sort * ltt)) =>
+           u0 = None /\ v = None \/
+           (exists (s : sort) (t : ltt) (g' : gtt),
+              u0 = Some (s, g') /\ v = Some (s, t) /\ projectionC g' q t)) lsg ys ->
+    exists Tq, onth n ys = Some(Sk, Tq) /\ projectionC x0 q Tq.
+Proof.
+  induction n; intros; try easy.
+  - destruct lsg; try easy.
+    destruct ys; try easy. simpl in *.
+    inversion H0. subst. destruct H4; try easy. 
+    destruct H. destruct H. destruct H. destruct H. destruct H1. inversion H. subst.
+    exists x1. split; try easy.
+  - destruct lsg; try easy.
+    destruct ys; try easy. simpl in *.
+    inversion H0. subst.
+    apply IHn with (lsg := lsg); try easy.
+Qed.
+
+Lemma _a_29_helper4 : forall n xs ys S' Sk T' x1,
+    onth n xs = Some (S', T') ->
+    onth n ys = Some (Sk, x1) ->
+    Forall2R
+        (fun u v : option (sort * ltt) =>
+         u = None \/
+         (exists (s s' : sort) (t t' : ltt),
+            u = Some (s, t) /\ v = Some (s', t') /\ subsort s s' /\ subtypeC t' t)) ys xs -> 
+    subtypeC T' x1.
+Proof.
+  induction n; intros.
+  - destruct xs; try easy. destruct ys; try easy.
+    inversion H1. subst. simpl in *. subst.
+    destruct H5; try easy. destruct H. destruct H. destruct H. destruct H. destruct H. destruct H0. destruct H2.
+    inversion H0. inversion H. subst. easy.
+  - destruct xs; try easy. destruct ys; try easy.
+    inversion H1. subst. specialize(IHn xs ys S' Sk). apply IHn; try easy.
+Qed.
+
+Lemma _a_29 : forall G p q PT QT S T S' T' xs n, 
+    wfgC G -> 
+    projectionC G p PT -> 
+    subtypeC (ltt_send q (extendLis n (Some (S, T)))) PT ->
+    projectionC G q QT -> 
+    onth n xs = Some (S', T') ->
+    subtypeC (ltt_recv p xs) QT -> 
+    exists G' ctxG SI Sn, 
+    typ_gtth ctxG G' G /\ (* 1 *)
+    (ishParts p G' -> False) /\ (ishParts q G' -> False) /\ (* 2 *)
+    List.Forall (fun u => u = None \/ (exists g lsg, u = Some g /\ g = gtt_send p q lsg /\
+      (exists s' Gjk Tp Tq, onth n lsg = Some (s', Gjk) /\ projectionC Gjk p Tp /\ subtypeC T Tp /\ projectionC Gjk q Tq /\ subtypeC T' Tq) /\
+      List.Forall2 (fun u v => (u = None /\ v = None) \/ (exists s g', u = Some(s, g') /\ v = Some s)) lsg SI
+    )) ctxG /\ (* 3 5 6 *)
+    (onth n SI = Some Sn) /\ subsort S Sn /\ subsort Sn S'. (* 5 6 *)
+Proof.
+  intros.
+  specialize(_a_29_10 G p q PT S T n H0 H1); intros.
+  destruct H5. destruct H5. destruct H5. destruct H5. destruct H6. destruct H7.
+  rename x0 into Sk. rename x1 into Tk.
+  specialize(proj_inj H0 H5); intros. subst. clear H5. (* _a_29_10 *)
+  
+  specialize(_a_29_11 G p q x H H0); intros.
+  destruct H5. destruct H5. destruct H5. destruct H9.
+  
+  rename x1 into ctxG. rename x0 into G'.
+  exists G'. exists ctxG.
+  assert (exists (SI : seq.seq (option sort)),
+    List.Forall2 (fun u v => (u = None /\ v = None) \/ (exists s t, u = Some s /\ v = Some (s, t))) SI x).
+  {
+    clear H H1 H0 H2 H3 H4 H8 H5 H6 H7 H9 H10. 
+    clear G p q QT S' T' T xs G' ctxG S n Sk Tk.
+    induction x; intros; try easy.
+    - exists []. easy.
+    - destruct IHx; try easy. destruct a.
+      - destruct p. exists (Some s :: x0). constructor; try easy.
+        right. exists s. exists l. easy.
+      - exists (None :: x0). constructor; try easy.
+        left. easy.
+  }
+  destruct H11 as [SI H11]. exists SI.
+  exists Sk. split. easy.
+  split. easy.
+  assert (onth n SI = Some Sk /\ subsort S Sk).
+  {
+    clear H1 H0 H10 H3.
+    revert H11 H6 H7. revert n x SI. induction n; intros; try easy.
+    - destruct SI; try easy. destruct x; try easy.
+      destruct x; try easy. inversion H11. subst.
+      simpl in H6. subst.
+      destruct H10; try easy. destruct H0. destruct H0. destruct H0. inversion H1. subst. easy.
+    - destruct SI; try easy. destruct x; try easy.
+      destruct x; try easy.
+      inversion H11. subst. simpl.
+      apply IHn with (x := x); try easy. 
+  }
+  specialize(_a_29_1314 G G' p q QT xs ctxG x H10 H5 H9 H2 H4); intros; try easy.
+  destruct H13. destruct H13. rename x0 into ys.
+  
+  specialize(proj_inj H13 H2); intros. subst. clear H13.
+  clear H7.
+  
+  specialize(_a_29_part ctxG G' G p q x ys H5 H0 H2 H9); intros.
+  split. easy.
+  assert (subsort Sk S').
+  {
+    clear H7 H12 H10 H9 H5 H8 H2 H0 H1 H.
+    specialize(subtype_recv_inv p xs ys H4); intros. clear H4.
+    revert H11 H14 H H3 H6. clear G p q S T G' ctxG.
+    revert S' T' xs x ys Sk Tk SI.
+    induction n; intros; try easy.
+    - destruct xs; try easy.
+      destruct x; try easy. 
+      destruct SI; try easy. destruct ys; try easy.
+      simpl in *.
+      subst.
+      inversion H14. subst. clear H14. inversion H11. subst. clear H11.
+      inversion H. subst. clear H.
+      destruct H4; try easy. destruct H. destruct H. destruct H. inversion H0. subst.
+      destruct H3; try easy. destruct H. destruct H. destruct H. destruct H. inversion H1. subst.
+      destruct H6; try easy. destruct H. destruct H. destruct H. destruct H. destruct H. destruct H2. destruct H3. 
+      inversion H. inversion H2. subst. easy.
+    - destruct xs; try easy.
+      destruct x; try easy.
+      destruct SI; try easy. destruct ys; try easy.
+      simpl in *. 
+      inversion H14. subst. clear H14. inversion H11. subst. clear H11.
+      inversion H. subst. clear H.
+      specialize(IHn S' T' xs x ys Sk Tk SI). apply IHn; try easy.
+  }
+  split; try easy.
+  
+  specialize(subtype_recv_inv p xs ys H4); intros.
+  specialize(subtype_send_inv q (extendLis n (Some (S, T))) x H1); intros.
+  
+  specialize(_a_29_16 G' ctxG G p q ys x H2 H10 H9 H7 H5); intros.
+  
+  specialize(Forall_forall (fun u : option gtt =>
+         u = None \/
+         (exists (g : gtt) (lsg : seq.seq (option (sort * gtt))),
+            u = Some g /\
+            g = gtt_send p q lsg /\
+            Forall2
+              (fun (u0 : option (sort * gtt)) (v : option (sort * ltt)) =>
+               u0 = None /\ v = None \/
+               (exists (s : sort) (t : ltt) (g' : gtt),
+                  u0 = Some (s, g') /\ v = Some (s, t) /\ projectionC g' p t)) lsg x /\
+            Forall2
+              (fun (u0 : option (sort * gtt)) (v : option (sort * ltt)) =>
+               u0 = None /\ v = None \/
+               (exists (s : sort) (t : ltt) (g' : gtt),
+                  u0 = Some (s, g') /\ v = Some (s, t) /\ projectionC g' q t)) lsg ys)) ctxG); intros.
+  destruct H18. specialize(H18 H17). clear H17 H19 H10.
+  
+  apply Forall_forall; intros.
+  specialize(H18 x0 H10). destruct H18. left. easy.
+  destruct H17. destruct H17. destruct H17. destruct H18. destruct H19.
+  right. exists (gtt_send p q x2). exists x2. subst.
+  split. easy. split. easy. 
+  rename x2 into lsg.
+  specialize(_a_29_helper n x Sk Tk lsg p H6 H19); intros. 
+  destruct H17. destruct H17.
+  specialize(_a_29_helper2 lsg SI x p H19 H11); intros. 
+  split; try easy. clear H21 H19.
+  exists Sk. exists x0. exists Tk.
+  specialize(_a_29_helper3 n lsg x0 Sk ys q H17 H20); intros.
+  destruct H19. destruct H19. exists x1. split. easy.
+  split. easy. split. easy. split. easy.
+  specialize(_a_29_helper4 n xs ys S' Sk T' x1); intros. apply H22; try easy.
+Qed.
+
+
+Lemma wfgC_after_step : forall G G' p q n, wfgC G -> gttstepC G G' p q n -> wfgC G'.
+Proof.
+Admitted.
+
+
+
+
+
 
 
