process/subject_reduction.v
@@ -9,27 +9,15 @@ Require Import Coq.Init.Datatypes.
 Inductive multiC : relation gtt := 
   | multiC_refl : forall G, multiC G G
   | multiC_step : forall G1 G2 G3 p q n, gttstepC G1 G2 p q n -> multiC G2 G3 -> multiC G1 G3.
-
-Lemma projection_cont_p : forall G x6 p q l x,
-    gttstepC G x6 q p l -> projectionC G p (ltt_recv q x) -> exists T, projectionC x6 p T.
-Proof.
   
-  
+Lemma step_mon : monotone5 gttstep.
 Admitted.
 
-Lemma projection_cont_q : forall G x6 p q l x0,
-    gttstepC G x6 q p l -> projectionC G q (ltt_send p x0) -> exists T, projectionC x6 q T.
-Admitted.
-
-Lemma projection_cont_r : forall G x6 q p0 l s x,
-    projectionC G s x ->
-    gttstepC G x6 q p0 l -> 
-    q <> s ->
-    p0 <> s ->
-    exists T, projectionC x6 s T.
+Lemma gttT_mon : monotone2 gttT.
 Admitted.
 
 Lemma projection_wfc_p : forall G l p q x4 x8 x9, 
+        wfgC G ->
         wfC (ltt_recv q x4) ->
         projectionC G p (ltt_recv q x4) ->
         gttstepC G x8 q p l ->
@@ -38,6 +26,7 @@ Lemma projection_wfc_p : forall G l p q x4 x8 x9,
 Admitted.
 
 Lemma projection_wfc_q : forall G l p q x x8 x9,
+        wfgC G ->
         wfC (ltt_send p x) ->
         projectionC G q (ltt_send p x) ->
         gttstepC G x8 q p l ->
@@ -46,6 +35,7 @@ Lemma projection_wfc_q : forall G l p q x x8 x9,
 Admitted.
 
 Lemma projection_wfc_r : forall G l p0 q s x x0 x6,
+        wfgC G ->
         wfC x ->
         q <> s ->
         p0 <> s ->
@@ -56,6 +46,7 @@ Lemma projection_wfc_r : forall G l p0 q s x x0 x6,
 Admitted.
 
 Lemma _3_19_h : forall p q l G L1 L2 S T xs y,
+  wfgC G ->
   projectionC G p (ltt_send q L1) -> 
   subtypeC (ltt_send q (extendLis l (Datatypes.Some(S,T)))) (ltt_send q L1) ->
   projectionC G q (ltt_recv p L2) -> 
@@ -70,15 +61,62 @@ Proof.
   - admit.
 Admitted.
 
-Lemma _3_19_1 : forall p q l G G' L1 L2 S T,
-  projectionC G p (ltt_send q L1) ->
-  subtypeC (ltt_send q (extendLis l (Datatypes.Some (S,T)))) (ltt_send q L1) ->
+Lemma _3_19_1 : forall p q l G G' LP LQ S T S' T' xs,
+  wfgC G ->
+  projectionC G p (ltt_send q LP) ->
+  subtypeC (ltt_send q (extendLis l (Datatypes.Some (S,T)))) (ltt_send q LP) ->
+  projectionC G q (ltt_recv p LQ) ->
+  onth l xs = Some (S', T') ->
+  subtypeC (ltt_recv p xs) (ltt_recv p LQ) ->
   gttstepC G G' p q l ->
-  projectionC G' p L2 ->
-  subtypeC T L2.
+  exists L, 
+  projectionC G' p L /\ subtypeC T L.
+Proof.
+  intros.
+  specialize(_a_29 G p q (ltt_send q LP) (ltt_recv p LQ) S T S' T' xs l H H0 H1 H2 H3 H4); intros.
+  destruct H6. rename x into Gl. revert H H0 H1 H2 H3 H4 H5 H6.
+  revert p q l G G' LP LQ S T S' T' xs.
+  induction Gl using gtth_ind_ref; intros; try easy.
+  - destruct H6. destruct H6. destruct H6. destruct H6. destruct H7. destruct H8. destruct H9. destruct H10. destruct H11.
+    inversion H6. subst.
+    specialize(some_onth_implies_In n x G H15); intros.
+    specialize(Forall_forall (fun u : option gtt =>
+         u = None \/
+         (exists (g : gtt) (lsg : list (option (sort * gtt))),
+            u = Some g /\
+            g = gtt_send p q lsg /\
+            (exists (s' : sort) (Gjk : gtt) (Tp Tq : ltt),
+               onth l lsg = Some (s', Gjk) /\
+               projectionC Gjk p Tp /\
+               subtypeC T Tp /\ projectionC Gjk q Tq /\ subtypeC T' Tq) /\
+            Forall2
+              (fun (u0 : option (sort * gtt)) (v : option sort) =>
+               u0 = None /\ v = None \/
+               (exists (s : sort) (g' : gtt), u0 = Some (s, g') /\ v = Some s)) lsg x0)) x); intros.
+    destruct H14. specialize(H14 H9). clear H9 H16.
+    specialize(H14 (Some G) H13). destruct H14; try easy.
+    destruct H9. destruct H9. destruct H9. destruct H14. destruct H16.
+    inversion H9. subst. 
+    destruct H16. destruct H14. destruct H14. destruct H14. destruct H14. destruct H16. destruct H18. destruct H19.
+    pinversion H5; try easy. subst.
+    specialize(eq_trans H30 H14); intros. inversion H21. subst. 
+    exists x5. split; try easy.
+    apply step_mon.
+  - destruct H7. destruct H7. destruct H7. destruct H7. destruct H8. destruct H9. destruct H10. destruct H11. destruct H12.
+    inversion H7. subst.
+    pinversion H1; try easy. 
+    - subst. admit.
+    - subst. 
+      assert (exists n t, onth n ys0 = Some t). { admit. }
+      destruct H14. destruct H14.
+      assert (exists g, onth x2 xs = Some g). { admit. }
+      
+      
+      
 Admitted.
 
 Lemma _3_19_2 : forall p q l G G' L1 L2 S T xs,
+  wfgC G ->
   projectionC G q (ltt_recv p L1) -> 
   subtypeC (ltt_recv p xs) (ltt_recv p L1) ->
   onth l xs = Some (S, T) ->
@@ -88,6 +126,7 @@ Lemma _3_19_2 : forall p q l G G' L1 L2 S T xs,
 Admitted.
 
 Lemma _3_19_3 : forall p q r l G G' L1 L2,
+  wfgC G ->
   r <> p -> r <> q ->
   projectionC G r L1 ->
   gttstepC G G' p q l -> 
@@ -96,27 +135,6 @@ Lemma _3_19_3 : forall p q r l G G' L1 L2,
 Proof.
   
 Admitted.
-
-Lemma onth_follow : forall l xs y x1,
-  onth l xs = Some y ->
-  Forall2
-       (fun (u : option process) (v : option (sort * ltt)) =>
-        u = None /\ v = None \/
-        (exists (p : process) (s : sort) (t : ltt),
-           u = Some p /\ v = Some (s, t) /\ typ_proc (Some s :: nil) nil p t))
-       xs x1 ->
-  exists s t, onth l x1 = Some (s, t).
-Proof.
-  induction l; intros; try easy.
-  destruct xs; subst. easy.
-  inversion H0; subst. clear H0. simpl in *. subst. 
-  - destruct H3. easy. destruct H. destruct H. destruct H. destruct H. destruct H0. inversion H. inversion H0. subst.
-    exists x0. exists x1. easy.
-  - destruct xs. easy.
-    destruct x1; try easy.
-    simpl in *.
-    inversion H0. subst. clear H0. apply IHl with (xs := xs) (y := y); try easy.
-Qed.
 
 Lemma _3_21_1_helper : forall l x1 xs x4 x5 y,
     onth l x1 = Some (x4, x5) ->
@@ -152,6 +170,7 @@ Proof.
 Qed.
 
 Lemma _3_21_3_helper : forall M p q x6 G l,
+    wfgC G ->
     ForallT
        (fun (u : string) (P : process) =>
         exists T : ltt, projectionC G u T /\ typ_proc nil nil P T) M ->
@@ -163,77 +182,61 @@ Lemma _3_21_3_helper : forall M p q x6 G l,
        exists T : ltt, projectionC x6 u T /\ typ_proc nil nil P T) M.
 Proof.
   intro M. induction M; intros; try easy.
-  - constructor; try easy.
-    inversion H. subst. destruct H4. destruct H3.
-    specialize(projection_cont_r G x6 q p0 l s x H3 H0); intros.
+  - constructor; try easy. 
+    inversion H0. subst. destruct H5. destruct H4.
+    specialize(projection_cont_r G x6 q p0 l s x H H4 H1); intros.
     assert (q <> s). { 
       unfold InT in H1. simpl in H1. 
-      specialize(Classical_Prop.not_or_and (s = q) False H1); intros. destruct H6.
+      specialize(Classical_Prop.not_or_and (s = q) False H2); intros. destruct H7.
       easy.
     }
     assert (p0 <> s). {
-      unfold InT in H2. simpl in H2.
-      specialize(Classical_Prop.not_or_and (s = p0) False H2); intros. destruct H7.
+      unfold InT in H3. simpl in H3.
+      specialize(Classical_Prop.not_or_and (s = p0) False H3); intros. destruct H8.
       easy.
     }
-    specialize(H5 H6 H7). destruct H5.
+    specialize(H6 H7 H8). destruct H6.
     exists x0.
     split; try easy.
     apply tc_sub with (t := x); try easy.
     specialize(_3_19_3 q p0 s l G x6 x x0); intros.
-    apply H8; try easy.
+    apply H9; try easy.
     assert (wfC x0). { 
         specialize(projection_wfc_r G l p0 q s x x0 x6); intros.
-        apply H8; try easy.
-        specialize(typable_implies_wfC H4). easy.
+        apply H9; try easy.
+        specialize(typable_implies_wfC H5). easy.
     } easy. 
-  - inversion H. subst. simpl in *.
+  - inversion H0. subst. simpl in *.
     unfold InT in *. simpl in *.
-    specialize(noin_cat_and q (flattenT M1) (flattenT M2) H1); intros.
-    specialize(noin_cat_and p (flattenT M1) (flattenT M2) H2); intros.
-    specialize(Classical_Prop.not_or_and (InT q M1) (InT q M2) H3); intros. destruct H7. 
-    specialize(Classical_Prop.not_or_and (InT p M1) (InT p M2) H4); intros. destruct H9.
+    specialize(noin_cat_and q (flattenT M1) (flattenT M2) H2); intros.
+    specialize(noin_cat_and p (flattenT M1) (flattenT M2) H3); intros.
+    specialize(Classical_Prop.not_or_and (InT q M1) (InT q M2) H4); intros. destruct H8. 
+    specialize(Classical_Prop.not_or_and (InT p M1) (InT p M2) H5); intros. destruct H10.
     constructor. apply IHM1 with (p := p) (q := q) (G := G) (l := l); try easy.
     apply IHM2 with (p := p) (q := q) (G := G) (l := l); try easy.
 Qed.
 
-Lemma _3_21_ssort_helper : forall l x x2 x3,
-      Forall2R
-        (fun u v : option (sort * ltt) =>
-         u = None \/
-         (exists (s s' : sort) (t t' : ltt),
-            u = Some (s, t) /\ v = Some (s', t') /\ subsort s s' /\ subtypeC t t'))
-        (extendLis l (Some (x2, x3))) x ->
-      exists y z, onth l x = (Some (y, z)) /\ subsort x2 y.
+Lemma _3_21_helper : forall l xs x1 y,
+    onth l xs = Some y ->
+    Forall2
+        (fun (u : option process) (v : option (sort * ltt)) =>
+         u = None /\ v = None \/
+         (exists (p : process) (s : sort) (t : ltt),
+            u = Some p /\
+            v = Some (s, t) /\ typ_proc (Some s :: nil) nil p t)) xs x1 ->
+    exists s t, onth l x1 = Some(s,t) /\ typ_proc (Some s :: nil) nil y t.
 Proof.
-  induction l; intros; try easy.
-  - destruct x; try easy. simpl in *.
-    destruct o. destruct p. exists s. exists l. split; try easy.
-    inversion H. subst. destruct H3; try easy. 
-    destruct H0. destruct H0. destruct H0. destruct H0. destruct H0. destruct H1. destruct H2.
-    inversion H0. inversion H1. subst. easy.
-    inversion H. subst. destruct H3; try easy.
-    destruct H0. destruct H0. destruct H0. destruct H0. destruct H0. destruct H1. easy.
-  - destruct x; try easy. simpl in *.
-    inversion H. subst. apply IHl with (x3 := x3); try easy.
+  induction l; intros.
+  - destruct xs; try easy.
+    destruct x1; try easy.
+    simpl in *.
+    inversion H0. subst. destruct H4; try easy. destruct H. destruct H. destruct H. destruct H. destruct H1. 
+    inversion H. subst.
+    exists x0. exists x2. split; try easy.
+  - destruct xs; try easy.
+    destruct x1; try easy. 
+    inversion H0. subst. apply IHl with (xs := xs); try easy.
 Qed.
-
-Lemma _3_21_ssort_helper2 : forall G p q x x8,
-      projectionC G p (ltt_recv q x8) ->
-      projectionC G q (ltt_send p x) ->
-      List.Forall2 (fun u v => (u = None /\ v = None) \/ (exists s t t', u = Some(s,t) /\ v = Some(s,t'))) x8 x.
-Proof.
-  
-Admitted.
-
-
-Lemma gttstep_wfc : forall G x8 q p l,
-    wfgC G ->
-    gttstepC G x8 q p l -> 
-    wfgC x8.
-Proof.
-    intros.
-Admitted.
 
 Theorem _3_21 : forall M M' G, typ_sess M G -> betaP M M' -> exists G', typ_sess M' G' /\ multiC G G'.
 Proof.
@@ -254,62 +257,67 @@ Proof.
     specialize(subtype_send x0 p (extendLis l (Some (x2, x3))) H17); intros.
     destruct H19. subst.
     specialize(subtype_send_inv p (extendLis l (Some (x2, x3))) x H17); intros.
-    specialize(_3_21_ssort_helper l x x2 x3 H19); intros.
-    destruct H20. destruct H20. destruct H20.
-  specialize(onth_follow l xs y x1 H H13); intros. destruct H22. destruct H22.
-  specialize(_3_19_h q p l G x x4 x2 x3 x1 (x6, x7) H5 H17 H1 H22 H12); intros. 
-  destruct H23. exists x8.
-  split.
-  specialize(wfgC_after_step G x8 q p l H23); intros. unfold wfgC in H24. (* flagged pf *)
-  destruct H24 as [G' H105].
-  apply t_sess with (Gl := G'); intros; try easy. 
-  - apply H2; try easy. 
-    admit.
-  - simpl in *. constructor. simpl.
-    apply Classical_Prop.and_not_or.
-    specialize(Classical_Prop.not_or_and (q = p) (In p (flattenT M)) H6); intros. destruct H20.
-    split; try easy. easy.
-  constructor. constructor. constructor.
-  - specialize(_3_19_2 q p l G x8); intros.
-    specialize(projection_cont_p G x8 p q l x4 H23 H1); intros.
-    destruct H25. 
-    specialize(H24 x4 x9 x6 x7 x1 H1 H12 H22 H23 H25). 
-    exists x9. split; try easy.
-    apply _a24 with (S := x6); try easy.
-    apply tc_sub with (t := x7); intros; try easy.
-    apply _3_21_1_helper with (l := l) (x1 := x1) (xs := xs); try easy.
-    assert(wfC x9). { 
-        specialize(projection_wfc_p G l p q x4 x8 x9); intros.
-        apply H26; try easy.
-        specialize(typable_implies_wfC H3). easy.
-    } 
-    easy.
-    assert(subsort x2 x6). { 
-      apply sstrans with (s2 := x0); try easy.
-      specialize(_3_21_ssort_helper2 G p q x x4 H1 H5); intros.
-      admit.
+  - specialize(_a_29 G q p (ltt_send p x) (ltt_recv q x4) x2 x3); intros.
+    specialize(_3_21_helper l xs x1 y H H13); intros.
+    destruct H21. destruct H21. destruct H21. 
+    specialize(H20 x0 x5 x1 l).
+    assert (wfgC G). 
+    {
+      unfold wfgC. exists Gl; try easy.
     }
-    apply sc_sub with (s := x2); try easy.
-    apply expr_typ_multi with (e := e); try easy.
-  - specialize(_3_19_1 q p l G x8 x); intros.
-    specialize(projection_cont_q G x8 p q l x H23 H5); intros.
-    destruct H25.
-    specialize(H24 x9 x2 x3 H5 H17 H23 H25).
-    constructor. exists x9. split; try easy.
-    apply tc_sub with (t := x3); try easy.
-    assert(wfC x9). { 
-          specialize(projection_wfc_q G l p q x x8 x9); intros.
-          apply H26; try easy.
-          specialize(typable_implies_wfC H10). easy.
-    } 
-    easy.
-  - apply _3_21_3_helper with (p := p) (q := q) (G := G) (l := l); try easy.
-    inversion H7. subst. easy.
-    simpl in H6. specialize(Classical_Prop.not_or_and (q = p) (In p (flattenT M)) H6); intros. 
-    destruct H20; try easy.
-  
-  apply multiC_step with (G2 := x8) (p := q) (q := p) (n := l). easy. apply multiC_refl.
-  
+    specialize(H20 H23 H5 H17 H1 H21 H12).
+    destruct H20. destruct H20. destruct H20. destruct H20. destruct H20. destruct H24. destruct H25. destruct H26. destruct H27.
+    destruct H28.
+    
+  - specialize(_3_19_h q p l G x x4 x2 x3 x1 (x0, x5) H23 H5 H17 H1 H21 H12); intros.
+    destruct H30. rename x10 into G'.
+    exists G'.
+    assert(multiC G G').
+    apply multiC_step with (G2 := G') (p := q) (q := p) (n := l). easy. apply multiC_refl.
+    split; try easy.
+    specialize(wfgC_after_step G G' q p l H23 H30); intros.
+    unfold wfgC in H32. destruct H32. rename x10 into Gl0.
+    apply t_sess with (Gl := Gl0); intros; try easy.
+    - apply H2; try easy.
+      admit. (* participant after gttstep is participant before step *)
+    - simpl in *.
+      constructor; try easy.
+    constructor. constructor. 
+    - constructor.
+      specialize(_3_19_2 q p l G G' x4); intros.
+      specialize(projection_cont_p G G' p q l x4 H23 H30 H1); intros.
+      destruct H34. exists x10. split; try easy.
+      specialize(H33 x10 x0 x5 x1 H23 H1 H12 H21 H30 H34).
+      apply _a24 with (S := x0); try easy.
+      - apply tc_sub with (t := x5); try easy.
+        assert (wfC x10). 
+        {
+          specialize(projection_wfc_p G l p q x4 G' x10); intros.
+          apply H35; try easy. 
+          specialize(typable_implies_wfC H3). easy.
+        }
+        easy.
+      - apply sc_sub with (s := x2); try easy.
+        apply expr_typ_multi with (e := e); intros; try easy.
+        apply sstrans with (s2 := x9); try easy.
+    - constructor.
+      specialize(_3_19_1 q p l G G' x); intros.
+      specialize(projection_cont_q G G' p q l x H23 H30 H5); intros.
+      destruct H34. exists x10. split; try easy.
+      specialize(H33 x10 x2 x3 H23 H5 H17 H30 H34).
+      apply tc_sub with (t := x3); try easy.
+      assert (wfC x10).
+      {
+        specialize(projection_wfc_q G l p q x G' x10); intros.
+        apply H35; try easy.
+        specialize(typable_implies_wfC H10). easy.
+      }
+      easy.
+    - apply _3_21_3_helper with (p := p) (q := q) (G := G) (l := l); try easy.
+      inversion H7. subst. easy.
+      simpl in H6. specialize(Classical_Prop.not_or_and (q = p) (In p (flattenT M)) H6); intros.
+      destruct H33; try easy. 
+
   (* T-COND *)
   inversion H0. subst. rename H3 into H100. rename H4 into H101. rename H5 into H102. rename H6 into H103. rename H7 into H3. 
   inversion H3. subst. clear H3.
